\begin{prof}{}{proof:complex:diff:exp}
To show that the function $f(t)=e^{z t}$ is differentiable, where $z=a+ ib$:
\begin{align*}
	f(t) = e^{zt}= e^{(a+ib)t}= e^{at}  e^{ib t}.
\end{align*}
The imaginary part of the complex number $e^{ib\cdot t}$ can be rewritten using \cref{eulers_form}:
\begin{align*}
	f(t) =& e^{at}\big(\cos(bt)+i \cdot \sin(bt)\big), \\
		 =& e^{at}\cos(bt) + e^{at} i \cdot \sin(bt).
\end{align*}
The rewritten function can be differentiated using the chain rule:
\begin{align}
	\dfrac{d}{dt}f(t) =& ae^{at}\cos(bt) -ib \cdot \sin(bt)e^{at} + ia \cdot e^{at}\sin(bt) + ib \cdot e^{at}\cos(bt), \nonumber \\
	=& e^{at} \bigg( a\big(\cos(bt) + i \cdot \sin(bt)\big) + b\big(i \cdot \cos(bt) - \sin(bt)\big) \bigg), \nonumber \\
	=& e^{at}\bigg(a \cdot e^{ib \cdot t}+b\big(i \cdot \cos(bt) - \sin(bt)\big)\bigg), \nonumber \\
	=& a e^{t(a+ib)} + b e^{at}\big(i \cdot \cos(bt) - \sin(bt)\big). \label{proof:chain}
\end{align}
Since $i^2 = -1$, \eqref{proof:chain} can be rewritten. Furthermore, $a+ib$ is replaced with $z$:
\begin{align*}
	\dfrac{d}{dt}f(t) =& a e^{zt} + b e^{at}\big(i \cdot \cos(bt) + i^2 \cdot \sin(bt)\big).
\end{align*}
$i$ is now moved outside the parentheses, and \cref{eulers_form} is used to reduce the equation:
\begin{align*}
	\dfrac{d}{dt}f(t) =&  a e^{zt} + ib e^{at}\big(\cos(bt) + i \cdot \sin(bt)\big), \\
	=&  a e^{zt} + ib e^{at}e^{ib \cdot t}. \\
\end{align*}
Now $a+ib$ is replaced with $z$, and $e^{zt}$ can be placed outside of the parentheses:
\begin{align*}
	\dfrac{d}{dt}f(t) =&  a e^{zt} + ib e^{t(a+ib)}, \\
	=&  e^{zt}(a+ib).
\end{align*}
$a+ib$ is again replaced with $z$, and \cref{theorem:complex:exp} is proved.
\end{prof}
